play around with bitvectors

theories/bitvector.v
@@ -1,5 +1,156 @@
 Require Export isla.base.
 
+Record bv (n : N) := BV {
+  bv_val : Z;
+  bv_in_range : -1 < bv_val < 2 ^ Z.of_N n;
+  (* TODO: Should we include the above?
+  Arguments for:
+  - all bit vectors are in normal form by construction and equivalence becomes eq
+    - can maybe be mitigated by normalizing aggressively
+  Arguments against:
+  - Makes constants annoying to write (needs tactics in terms which seems to break stuff in weird ways, e.g typeclass search)
+  - n1 = n2 cannot be long solved by done
+  *)
+}.
+Arguments bv_val {_}.
+
+Global Program Instance bv_eq_dec n : EqDecision (bv n) := λ '(BV _ v1 p1) '(BV _ v2 p2),
+   match decide (v1 = v2) with
+   | left eqv => left _
+   | right eqv => right _
+   end.
+Next Obligation. move => *. subst. f_equal. apply: proof_irrel. Qed.
+Next Obligation. move => * [?]. done. Qed.
+
+Lemma bv_eq n (b1 b2 : bv n) :
+  b1 = b2 ↔ b1.(bv_val) = b2.(bv_val).
+Proof. destruct b1, b2. split => /=; first by case. move => ?. subst. f_equal => //. apply: proof_irrel. Qed.
+
+Coercion bv_val : bv >-> Z.
+
+Definition bv_of_Z_checked (n : N) (z : Z) : option (bv n) :=
+  match decide (-1 < z < 2 ^ Z.of_N n) with
+  | left Heq => Some (BV n z Heq)
+  | right _ => None
+  end.
+
+Record bvn := BVN {
+  bvn_n : N;
+  bvn_val : bv bvn_n;
+}.
+
+Lemma bvn_eq (b1 b2 : bvn) :
+  b1 = b2 ↔ b1.(bvn_n) = b2.(bvn_n) ∧ b1.(bvn_val).(bv_val) = b2.(bvn_val).(bv_val).
+Proof.
+  split; [ naive_solver|]. destruct b1, b2 => /= -[??]. subst. f_equal.
+  by apply/bv_eq.
+Qed.
+
+Global Program Instance bvn_eq_dec : EqDecision bvn := λ '(BVN n1 b1) '(BVN n2 b2),
+   match decide (n1 = n2) with
+   | left eqv => match decide (b1.(bv_val) = b2.(bv_val)) with
+                | left eqb => left _
+                | right eqb => right _
+                end
+   | right eqv => right _
+   end.
+Next Obligation. move => *. apply/bvn_eq. naive_solver. Qed.
+Next Obligation. move => *. apply/bvn_eq. naive_solver. Qed.
+Next Obligation. move => *. apply/bvn_eq. naive_solver. Qed.
+
+Definition bvn_to_bv (n : N) (b : bvn) : option (bv n) :=
+  match decide (b.(bvn_n) = n) with
+  | left eq => Some (eq_rect (bvn_n b) (λ n0 : N, bv n0)
+           (bvn_val b) n eq)
+  | right _ => None
+  end.
+Arguments bvn_to_bv !_ !_ /.
+
+Definition bv_to_bvn {n} (b : bv n) : bvn := BVN _ b.
+Coercion bv_to_bvn : bv >-> bvn.
+
+Ltac solve_bitvector_eq :=
+  try (vm_compute; done);
+  lazymatch goal with
+  | |- -1 < ?v < 2 ^ ?l =>
+    fail "Bitvector constant" v "does not fit into" l "bits"
+  end.
+
+Notation "'[BV{' l } v ]" := (BV l v _) (at level 9, format "[BV{ l }  v ]", only printing) : stdpp_scope.
+Notation "'[BV{' l } v ]" := (BV l v ltac:(solve_bitvector_eq)) (at level 9, only parsing) : stdpp_scope.
+(* Notation "'[BV{' l } v ]" := (BV l v) (at level 9, format "[BV{ l }  v ]") : stdpp_scope. *)
+
+Goal ([BV{10} 3 ] = [BV{10} 5]). Abort.
+Fail Goal ([BV{2} 3 ] = [BV{10} 5]).
+Goal ([BV{2} 3 ] =@{bvn} [BV{10} 5]). Abort.
+Fail Goal ([BV{2} 4 ] = [BV{2} 5]).
+Goal bvn_to_bv 2 [BV{2} 3] = Some [BV{2} 3]. done. Abort.
+
+
+Program Definition bv_zero_extend {n} (z : N) (b : bv n) : bv (n + z) := {|
+  bv_val := b.(bv_val);
+|}.
+Next Obligation. Admitted.
+
+Definition Z_to_signed (bits n : Z) : Z :=
+  if bool_decide (2 ^ (bits - 1) ≤ n) then
+    n - 2 ^ bits
+  else
+    n.
+
+Definition Z_to_unsigned (bits n : Z) : Z :=
+  if bool_decide (n ≤ 0) then
+    n + 2 ^ bits
+  else
+    n.
+
+Program Definition bv_sign_extend {n} (z : N) (b : bv n) : bv (n + z) := {|
+  bv_val := Z_to_unsigned (Z.of_N (n + z)) (Z_to_signed (Z.of_N n) b.(bv_val))
+|}.
+Next Obligation. Admitted.
+
+
+(* s is start, l is len *)
+Program Definition bv_extract {n} (s l : N) (b : bv n) : bv (l) := {|
+  bv_val := Z.land (b.(bv_val) ≫ Z.of_N s) (Z.ones (Z.of_N l));
+|}.
+Next Obligation. Admitted.
+
+Program Definition bv_add {n} (b1 b2 : bv n) : bv n := {|
+  bv_val := b1.(bv_val) + b2.(bv_val) `mod` 2 ^ Z.of_N n;
+|}.
+Next Obligation. Admitted.
+
+Program Definition bv_or {n} (n1 n2 : bv n) : bv n := {|
+  bv_val := Z.lor n1.(bv_val) n2.(bv_val);
+|}.
+Next Obligation. Admitted.
+
+Program Definition bv_and {n} (n1 n2 : bv n) : bv n := {|
+  bv_val := Z.land n1.(bv_val) n2.(bv_val);
+|}.
+Next Obligation. Admitted.
+
+Program Definition bv_not {n} (b : bv n) : bv n := {|
+  bv_val := Z_lunot (Z.of_N n) b.(bv_val);
+|}.
+Next Obligation. Admitted.
+
+Program Definition bv_concat {n1 n2} (b1 : bv n1) (b2 : bv n2) : bv (n1 + n2) := {|
+  (* TODO: Is this the right way around? *)
+  bv_val := Z.lor (b1.(bv_val) ≪ Z.of_N n2) b2.(bv_val);
+|}.
+Next Obligation. Admitted.
+
+Program Definition bv_shr {n} (n1 n2 : bv n) : bv n := {|
+  (* TODO: Is this the right way around? *)
+  bv_val := (n1.(bv_val) ≫ n2.(bv_val));
+|}.
+Next Obligation. Admitted.
+
+
+(*
+(*** Old definition of bit vectors *)
 
 Record bv := BV {
   bv_len : Z;
@@ -90,3 +241,4 @@ Program Definition bv_shr (n1 n2 : bv) : bv := {|
   (* TODO: Is this the right way around? *)
   bv_val := (n1.(bv_val) ≫ n2.(bv_val));
 |}.
+*)
